
Motorboat is moving. Drag force given as $-kv$.

\bigbreak Given:
\begin{itemize}
    \item $ m = 3000\,kg $
    \item $ \vec{F_d} = -k\vec{v} $
    \item $ k = 100\,kg/s $
    \item $ v(33) = 2\,m/s $
\end{itemize}


\bigbreak Questions:
\begin{itemize}
    \item Find the maximum speed the boat can reach
\end{itemize}


\subsection*{Solution}
\subsubsection*{Derivations}

The net force could be expressed as:

$$ F_{net} = F_{engine} - F_{drag} $$
$$ F_{net} = F_{engine} - kv $$

Newton's law:

$$ F_{net} = m \frac{dv}{dt} $$

Therefore:

$$ F_{engine} - kv = m \frac{dv}{dt}  $$

\bigbreak Let us divide the equation by $m$:

$$ \frac{F_{engine}}{m} - \frac{kv}{m} = \frac{dv}{dt}  $$
\begin{equation}
    \label{eq:diffur}
    \frac{dv}{dt} + \frac{k}{m}v = \frac{F_{engine}}{m}
\end{equation}

\bigbreak Above we just got a first-order liner differential equation. Let us find the integrating factor.

$$ \mu(t) = e ^ {\int \frac{k}{m} dt} = e^{\frac{k}{m}t} $$ 

\bigbreak Now as we found the integrating factor, we can mul \ref{eq:diffur} by it.

$$ e^{\frac{k}{m}t} \frac{dv}{dt} + e^{\frac{k}{m}t} \frac{k}{m}v = e^{\frac{k}{m}t} \frac{F_{engine}}{m} $$
$$ \frac{d}{dt}(e^{\frac{k}{m}t} \cdot v) = \frac{F_{engine}}{m} e^{\frac{k}{m}t} $$

\bigbreak Now we simply integrate both sides (with respect to t):

$$ \int\frac{d}{dt}(e^{\frac{k}{m}t} \cdot v) dt = \int \frac{F_{engine}}{m} e^{\frac{k}{m}t} dt $$
$$ e^{\frac{k}{m}t} \cdot v = \frac{F_{engine}}{k} e^{\frac{k}{m}t} + C $$
\begin{equation}
    \label{eq:velocity}
    v(t) = \frac{F_{engine}}{k} + \frac{C}{e^{\frac{k}{m}t}}
\end{equation}

\subsubsection*{Substitution}

\bigbreak Now let us apply initial conditions at \ref{eq:velocity}:
\bigbreak At $t = 0$, $v(0) = 0$:

$$ 0 = \frac{F_{engine}}{k} + C $$
$$ C = - \frac{F_{engine}}{k} $$

Reformat \ref{eq:velocity}:

$$ v(t) = \frac{F_{engine}}{k} + \frac{- \frac{F_{engine}}{k}}{e^{\frac{k}{m}t}} $$
$$ v(t) = \frac{F_{engine}}{k} (1 -  \frac{1}{e^{\frac{k}{m}t}}) $$

\bigbreak At $t = 33$, $v(33) = 2m/s$:

$$ 2m/s = \frac{F_{engine}}{k} (1 -  \frac{1}{e^{\frac{k}{m}33}}) $$
$$ 2m/s = \frac{F_{engine}}{100kg/s} (1 -  \frac{1}{e^{\frac{100kg/s}{3000kg}33}}) $$

Solve for $F_{engine}$:

$$ F_{engine} = \frac{2m/s \cdot 100kg/s}{1 -  \frac{1}{e^{\frac{100kg/s}{3000kg}33}}} \approx 299.9N$$

\bigbreak \ref{eq:velocity} Maximal velocity reaches when $ t \rightarrow \infty $
\smallbreak Then $ C \rightarrow 0 $

\bigbreak Hence:

$$ v_{max} = \frac{F_{engine}}{k} = \frac{299.9N}{100kg/s} = \boxed{2.9m/s} $$

\vfill \subsection*{ANSWER}
\begin{itemize}
    \item $3m/s$
\end{itemize}